

[u_0 u_1 u_2 u_3]
[y_0 y_1 y_2 y_3] ⁎ [c_0 c_1 c_2]

y_0 = u_0
y_1 = c_0 y_0 + u_1
y_2 = c_0 y_1 + c_1 y_0 + u_2
y_3 = c_0 y_2 + c_1 y_1 + c_2 y_0 + u_3

∂E/∂c_0 = ∂E/∂y_0 ∂y_0/∂c_0 + ∂E/∂y_1 ∂y_1/∂c_0 + ∂E/∂y_2 ∂y_2/∂c_0 + ∂E/∂y_3 ∂y_3/∂c_0
        =                     ∂E/∂y_1 y_0       + ∂E/∂y_2 y_1       + ∂E/∂y_3 y_2

∂E/∂c_1 = ∂E/∂y_0 ∂y_0/∂c_1 + ∂E/∂y_1 ∂y_1/∂c_1 + ∂E/∂y_2 ∂y_2/∂c_1 + ∂E/∂y_3 ∂y_3/∂c_1
        =                                         ∂E/∂y_2 y_0       + ∂E/∂y_3 y_1

∂E/∂c_2 = ∂E/∂y_0 ∂y_0/∂c_2 + ∂E/∂y_1 ∂y_1/∂c_2 + ∂E/∂y_2 ∂y_2/∂c_2 + ∂E/∂y_3 ∂y_3/∂c_2
        =                                                             ∂E/∂y_3 y_0

[∂E/∂y_0 ∂E/∂y_1 ∂E/∂y_2 ∂E/∂y_3] ⁎ [y_0 y_1 y_2 y_3]

                         ∂E/∂y_3 y_0
                 ∂E/∂y_2 y_0 + ∂E/∂y_3 y_1
         ∂E/∂y_1 y_0 + ∂E/∂y_2 y_1 + ∂E/∂y_3 y_2

4 - 1 = 3

[1 2 3 4] * [1 2 3]
1 3 8 21

dedc0 = 1 1 + 1 3 + 1 8 = 12 - 19 = -7
dedc1 = 0 + 1 1 + 1 3 = 4 - 5 = -1
dedc2 = 0 + 0 + 1 1 = 1 - 1 = 0
